proof/invariant-abstract/RISCV64/ArchVSpace_AI.thy
@@ -928,7 +928,7 @@ lemma is_final_cap_caps_of_state_2D:
                         prod_eqI)
   done
 
-crunch underlying_memory[wp]: ackInterrupt, hwASIDFlush, read_stval, setVSpaceRoot, sfence
+crunch underlying_memory[wp]: ackInterrupt, hwASIDFlush, read_stval, setVSpaceRoot, sfence, tfence
   "\<lambda>m'. underlying_memory m' p = um"
   (simp: cache_machine_op_defs machine_op_lift_def machine_rest_lift_def split_def)
 
